inference-tool/src/main/scala/inference/FrontEnd.scala
@@ -9,20 +9,26 @@ import scopt.OParser
 
 object Heuristics extends Enumeration {
   type Heuristic = Value
-  val store, inc, same, ignore = Value
+  val store, inc, same, ignore, ignoret = Value
+}
+
+object Nondeterminisms extends Enumeration {
+  type Nondeterminism = Value
+  val basic, labar = Value
 }
 
 object FrontEnd {
-  type UpdateModifier = Nat.nat => (Nat.nat => (Nat.nat => (FSet.fset[(Nat.nat, ((Nat.nat, Nat.nat), Transition.transition_ext[Unit]))] => (FSet.fset[(Nat.nat, ((Nat.nat, Nat.nat), Transition.transition_ext[Unit]))] => Option[FSet.fset[(Nat.nat, ((Nat.nat, Nat.nat), Transition.transition_ext[Unit]))]]))))
-
   implicit val heuristicsRead: scopt.Read[Heuristics.Value] =
-  scopt.Read.reads(Heuristics withName _)
+    scopt.Read.reads(Heuristics withName _)
+  implicit val nondeterminismsRead: scopt.Read[Nondeterminisms.Value] =
+    scopt.Read.reads(Nondeterminisms withName _)
 
   def main(args: Array[String]): Unit = {
     case class Config(
       heuristics: Seq[Heuristics.Heuristic] = Seq(),
       file: File = null,
-      outputname: String = null
+      outputname: String = null,
+      nondeterminism: Nondeterminisms.Nondeterminism = Nondeterminisms.basic
     )
 
     val builder = OParser.builder[Config]
@@ -35,11 +41,15 @@ object FrontEnd {
         opt[Seq[Heuristics.Heuristic]]('h', "heuristics")
           .valueName("<heuristic1>,<heuristic2>...")
           .action((x, c) => c.copy(heuristics = x))
-          .text("heuristics to give the inference process (store,inc,same,ignore)"),
+          .text(s"heuristics to give the inference process ${Heuristics.values}"),
         opt[String]('o', "output")
           .valueName("filename")
           .action((x, c) => c.copy(outputname = x))
           .text("The preferred name of the file to output the SAL and DOT representations of the inferred model to - defaults to the input file name"),
+        opt[Nondeterminisms.Nondeterminism]('n', "nondeterminism")
+          .valueName("nondeterminism checker")
+          .action((x, c) => c.copy(nondeterminism = x))
+          .text(s"The preferred definition of nondeterminism - defaults to label, arity, and guard check ${Nondeterminisms.values}"),
         arg[File]("filename")
           .required()
           .action((x, c) => c.copy(file = x))
@@ -47,6 +57,7 @@ object FrontEnd {
     }
 
     println("=================================================================")
+    val t1 = System.nanoTime
     OParser.parse(parser1, args, Config()) match {
       case Some(config) =>
         val rawJson = Source.fromFile(config.file).getLines.mkString
@@ -54,20 +65,30 @@ object FrontEnd {
         val list = parsed.values.asInstanceOf[List[List[Map[String, Any]]]]
         val log = list.map(run => run.map(x => TypeConversion.toEventTuple(x)))
 
-        val heuristics = scala.collection.immutable.Map[Heuristics.Heuristic, UpdateModifier](
+        val heuristics = scala.collection.immutable.Map(
           Heuristics.store -> Store_Reuse.heuristic_1(log),
           Heuristics.inc -> (Increment_Reset.insert_increment_2 _).curried,
           Heuristics.same -> (Same_Register.same_register _).curried,
-          Heuristics.ignore -> (Ignore_Inputs.drop_inputs _).curried
+          Heuristics.ignore -> (Ignore_Inputs.drop_inputs _).curried,
+          Heuristics.ignoret -> (Ignore_Inputs.transitionwise_drop_inputs _).curried
         )
 
-        val inferred = Inference.learn(log, (SelectionStrategies.naive_score_one_final_state _).curried, Inference.try_heuristics(config.heuristics.map(x => heuristics(x)).toList))
+        val nondeterminisms = scala.collection.immutable.Map(
+          Nondeterminisms.basic -> (Inference.nondeterministic_pairs _),
+          Nondeterminisms.labar -> (Inference.nondeterministic_pairs_labar _)
+        )
+
+        val inferred = Inference.learn(
+          log,
+          (SelectionStrategies.naive_score_one_final_state _).curried,
+          Inference.try_heuristics(config.heuristics.map(x => heuristics(x)).toList, nondeterminisms(config.nondeterminism)),
+          nondeterminisms(config.nondeterminism))
 
         inferred match {
           case None => println("No EFSM could be inferred")
           case Some(inferred) => {
             println("The inferred machine is " +
-              (if (Inference.nondeterministic(Inference.toiEFSM(inferred))) "non" else "") + "deterministic")
+              (if (Inference.nondeterministic(Inference.toiEFSM(inferred), Inference.nondeterministic_pairs)) "non" else "") + "deterministic")
 
             val basename = (if (config.outputname == null) (FilenameUtils.getBaseName(config.file.getName()).replace("-", "_")) else config.outputname.replace("-", "_"))
 
@@ -78,7 +99,10 @@ object FrontEnd {
       case _ =>
         System.exit(1)
     }
-
+    val seconds = (System.nanoTime - t1) / 1e9d
+    val minutes = (seconds/60)%60
+    val hours = seconds/3600
+    println(s"Completed in ${if (hours > 0) s"${hours}h " else ""}${if (minutes > 0) s"${minutes}m " else ""}${seconds%60}s")
     println("=================================================================")
   }
 }
