formal/Contexts.thy
@@ -13,8 +13,10 @@ begin
 declare gval.simps [simp]
 declare ValueEq_def [simp]
 
-definition can_take :: "transition \<Rightarrow> inputs \<Rightarrow> registers \<Rightarrow> bool" where
-  "can_take t i r = (length i = Arity t \<and> apply_guards (Guard t) (join_ir i r))"
+definition can_take :: "nat \<Rightarrow> gexp list \<Rightarrow> inputs \<Rightarrow> registers \<Rightarrow> bool" where
+  "can_take a g i r = (length i = a \<and> apply_guards g (join_ir i r))"
+
+definition "can_take_transition t i r = can_take (Arity t) (Guard t) i r"
 
 lemma enumerate_gexp_regs_set_reg_unconstrained:
   "\<forall>x\<in>set G. enumerate_gexp_regs x = {} \<Longrightarrow>
@@ -606,10 +608,13 @@ next
     by (metis (no_types, hide_lams) take_eq_Nil test_aux_aux value_minus.simps(2) value_minus.simps(4) zero_le)
 qed
 
-lemma medial_subset: "length i = Arity t \<Longrightarrow>
-                      Arity t = Arity t' \<Longrightarrow>
-                      set (Guard t') \<subseteq> set (Guard t) \<Longrightarrow> can_take t i r \<longrightarrow> can_take t' i r"
-  by (simp add: can_take_def apply_guards_subset)
+lemma medial_subset:
+  "length i = Arity t \<Longrightarrow>
+  Arity t = Arity t' \<Longrightarrow>
+  set (Guard t') \<subseteq> set (Guard t) \<Longrightarrow>
+  can_take_transition t i r \<Longrightarrow>
+  can_take_transition t' i r"
+  by (simp add: can_take_transition_def can_take_def apply_guards_subset)
 
 definition d2r :: "datastate \<Rightarrow> registers" where
   "d2r d = (\<lambda>r. d (R r))"
@@ -617,47 +622,57 @@ definition d2r :: "datastate \<Rightarrow> registers" where
 lemma d2r_keeps_regs_same [simp]: "d2r c r = c (R r)"
   by (simp add: d2r_def)
 
+definition posterior_separate :: "nat \<Rightarrow> gexp list \<Rightarrow> update_function list \<Rightarrow> inputs \<Rightarrow> registers \<Rightarrow> registers option" where
+  "posterior_separate a g u i r = (if can_take a g i r then Some (apply_updates u (join_ir i r) r) else None)"
+
 definition posterior :: "transition \<Rightarrow> inputs \<Rightarrow> registers \<Rightarrow> registers option" where
-  "posterior t i r = (if can_take t i r then Some (apply_updates (Updates t) (join_ir i r) r) else None)"
+  "posterior t i r = posterior_separate (Arity t) (Guard t) (Updates t) i r"
 
 definition r2d :: "registers \<Rightarrow> datastate" where
   "r2d regs = (\<lambda>i. case i of R r \<Rightarrow> regs r | _ \<Rightarrow> None)"
 
 definition subsumes :: "transition \<Rightarrow> registers \<Rightarrow> transition \<Rightarrow> bool" where
   "subsumes t2 r t1 = (Label t1 = Label t2 \<and> Arity t1 = Arity t2 \<and>
-                       (\<forall>i. can_take t1 i r \<longrightarrow> can_take t2 i r) \<and>
-                       (\<forall>i. can_take t1 i r \<longrightarrow> apply_outputs (Outputs t1) (join_ir i r) = apply_outputs (Outputs t2) (join_ir i r)) \<and>
-                       (\<forall>p1 p2 i. posterior t2 i r = Some p2 \<and> posterior t1 i r = Some p1 \<longrightarrow> (\<forall>P r'. (p1 r' = None) \<or> (P (p2 r') \<longrightarrow> P (p1 r')))) \<and>
+                       (\<forall>i. can_take_transition t1 i r \<longrightarrow> can_take_transition t2 i r) \<and>
+                       (\<forall>i. can_take_transition t1 i r \<longrightarrow> apply_outputs (Outputs t1) (join_ir i r) = apply_outputs (Outputs t2) (join_ir i r)) \<and>
+                       (\<forall>p1 p2 i. posterior_separate (Arity t2) ((Guard t2)@(Guard t1)) (Updates t2) i r = Some p2 \<and>
+                                  posterior_separate (Arity t1) (Guard t1) (Updates t1) i r = Some p1 \<longrightarrow>
+                                  (\<forall>P r'. (p1 r' = None) \<or> (P (p2 r') \<longrightarrow> P (p1 r')))) \<and>
                        (\<forall>p1 p2 i. posterior t2 i r = Some p2 \<and> posterior t1 i r = Some p1 \<longrightarrow> (\<forall>r. p1 r \<noteq> None \<longrightarrow>  p2 r \<noteq> None))
                       )"
 
 lemma subsumption: 
   "(Label t1 = Label t2 \<and> Arity t1 = Arity t2) \<Longrightarrow>
-   (\<forall>i. can_take t1 i r \<longrightarrow> can_take t2 i r) \<Longrightarrow>
-   (\<forall>i. can_take t1 i r \<longrightarrow> apply_outputs (Outputs t1) (join_ir i r) = apply_outputs (Outputs t2) (join_ir i r)) \<Longrightarrow>
-   (\<forall>p1 p2 i. posterior t2 i r = Some p2 \<and> posterior t1 i r = Some p1 \<longrightarrow> (\<forall>P r'. (p1 r' = None) \<or> (P (p2 r') \<longrightarrow> P (p1 r')))) \<Longrightarrow>
+   (\<forall>i. can_take_transition t1 i r \<longrightarrow> can_take_transition t2 i r) \<Longrightarrow>
+   (\<forall>i. can_take_transition t1 i r \<longrightarrow> apply_outputs (Outputs t1) (join_ir i r) = apply_outputs (Outputs t2) (join_ir i r)) \<Longrightarrow>
+   (\<forall>p1 p2 i. posterior_separate (Arity t2) ((Guard t2)@(Guard t1)) (Updates t2) i r = Some p2 \<and>
+                                  posterior_separate (Arity t1) (Guard t1) (Updates t1) i r = Some p1 \<longrightarrow>
+                                  (\<forall>P r'. (p1 r' = None) \<or> (P (p2 r') \<longrightarrow> P (p1 r')))) \<Longrightarrow>
    (\<forall>p1 p2 i. posterior t2 i r = Some p2 \<and> posterior t1 i r = Some p1 \<longrightarrow> (\<forall>r. p1 r \<noteq> None \<longrightarrow>  p2 r \<noteq> None)) \<Longrightarrow>
    subsumes t2 r t1"
   by (simp add: subsumes_def)
 
-lemma bad_guards: "\<exists>i. can_take t1 i r \<and> \<not> can_take t2 i r \<Longrightarrow> \<not> subsumes t2 r t1"
+lemma bad_guards: "\<exists>i. can_take_transition t1 i r \<and> \<not> can_take_transition t2 i r \<Longrightarrow> \<not> subsumes t2 r t1"
   by (simp add: subsumes_def)
 
 lemma inconsistent_updates: "\<exists>p1 p2. (\<exists>i. posterior t2 i r = Some p2 \<and> posterior t1 i r = Some p1) \<and> (\<exists>r. (\<exists>y. p1 r = Some y) \<and> p2 r = None) \<Longrightarrow>
  \<not> subsumes t2 r t1"
   by (simp add: subsumes_def)
 
-lemma inconsistent_updates2: "\<exists>p1 p2. (\<exists>i. posterior t2 i r = Some p2 \<and> posterior t1 i r = Some p1) \<and> (\<exists>P r'. P (p2 r') \<and> (\<exists>y. p1 r' = Some y) \<and> \<not> P (p1 r')) \<Longrightarrow>
- \<not> subsumes t2 r t1"
+lemma inconsistent_updates2: "\<exists>p1 p2.
+       (\<exists>i. posterior_separate (Arity t2) (Guard t2 @ Guard t1) (Updates t2) i r = Some p2 \<and>
+            posterior_separate (Arity t1) (Guard t1) (Updates t1) i r = Some p1) \<and>
+       (\<exists>P r'. P (p2 r') \<and> (\<exists>y. p1 r' = Some y) \<and> \<not> P (p1 r')) \<Longrightarrow>
+    \<not> subsumes t2 r t1"
   by (simp add: subsumes_def)
 
-lemma bad_outputs: "\<exists>i. can_take t1 i r \<and> apply_outputs (Outputs t1) (join_ir i r) \<noteq> apply_outputs (Outputs t2) (join_ir i r) \<Longrightarrow>
+lemma bad_outputs: "\<exists>i. can_take_transition t1 i r \<and> apply_outputs (Outputs t1) (join_ir i r) \<noteq> apply_outputs (Outputs t2) (join_ir i r) \<Longrightarrow>
  \<not> subsumes t2 r t1"
   by (simp add: subsumes_def)
 
 lemma transition_subsumes_self: "subsumes t c t"
   apply (simp add: subsumes_def)
-  by auto
+  using posterior_separate_def by auto
 
 primrec posterior_sequence :: "transition_matrix \<Rightarrow> cfstate \<Rightarrow> registers \<Rightarrow> trace \<Rightarrow> registers option" where
   "posterior_sequence _ _ r [] = Some r" |
@@ -716,4 +731,24 @@ lemma accepts_trace_gives_context: "accepts_trace e p \<Longrightarrow> (\<exist
 
 lemma accepts_trace_anterior_not_none: "accepts_trace e p \<Longrightarrow> anterior_context e p \<noteq> None"
   using accepts_trace_gives_context by blast
+
+lemma mutually_exclusive_not_apply_guards:
+  "\<not> satisfiable (fold gAnd (G1 @ G2) (Bc True)) \<Longrightarrow>
+   apply_guards G1 (join_ir i c) \<Longrightarrow>
+   \<not> apply_guards G2 (join_ir i c)"
+  apply (simp only: fold_apply_guards satisfiable_def)
+  apply (simp add: apply_guards_def)
+  by blast
+
+lemma "\<exists>i. can_take_transition t1 i c \<Longrightarrow>
+       \<not>satisfiable (fold gAnd ((Guard t1)@(Guard t2)) (Bc True)) \<Longrightarrow>
+       \<not> subsumes t2 c t1"
+  apply (simp add: subsumes_def del: fold_append)
+  apply standard
+  apply standard
+  apply (rule disjI1)
+  apply clarify
+  apply (rule_tac x=i in exI)
+  by (simp add: can_take_transition_def can_take_def mutually_exclusive_not_apply_guards)
+
 end
