formal/inference/heuristics/Ignore_Inputs.thy
@@ -5,17 +5,39 @@ begin
 definition enumerate_outputs :: "iEFSM \<Rightarrow> label \<Rightarrow> arity \<Rightarrow>  aexp list fset" where
   "enumerate_outputs e l a = (fimage (\<lambda>(_, _, t). Outputs t) (ffilter (\<lambda>(_, _, t). Label t = l \<and> Arity t = a) e))"
 
+definition drop_guards :: "transition \<Rightarrow> transition" where
+  "drop_guards t = \<lparr>Label = Label t, Arity = Arity t, Guard = [], Outputs = Outputs t, Updates = Updates t\<rparr>"
+
 definition drop_inputs :: "update_modifier" where
-  "drop_inputs t1ID t2ID s new old = (let
+  "drop_inputs t1ID t2ID s new old np = (let
      t1 = (get_by_id new t1ID);
      t2 = (get_by_id new t2ID) in
      if fis_singleton (enumerate_outputs new (Label t1) (Arity t1)) then
      Some (fimage 
       (\<lambda>(id, route, t). 
        if id = t1ID then
-         (id, route, \<lparr>Label = Label t, Arity = Arity t, Guard = [], Outputs = Outputs t, Updates = Updates t\<rparr>)
+         (id, route, drop_guards t)
        else (id, route, t)) (ffilter (\<lambda>(id, _). id \<noteq> t2ID) new))
      else None
    )"
+
+definition transitionwise_drop_inputs :: update_modifier where
+  "transitionwise_drop_inputs t1ID t2ID s new old np = (let
+     t1 = (get_by_id new t1ID);
+     t2 = (get_by_id new t2ID) in
+     if Outputs t1 = Outputs t2 then
+       Some (replace (drop_transition new t2ID) t1ID (drop_guards t1))
+     else
+       None)"
+
+lemma drop_inputs_subsumption: "subsumes (drop_guards t1) c t1"
+  apply (rule subsumption)
+      apply (simp add: drop_guards_def)
+     apply (simp add: drop_guards_def can_take_def can_take_transition_def)
+    apply (simp add: drop_guards_def)
+   apply (simp add: drop_guards_def posterior_separate_def)
+   apply auto[1]
+  apply (simp add: drop_guards_def posterior_def posterior_separate_def)
+  by auto
 
 end
